\begin{frame}
    \frametitle{Quantum Mechanics Abstract}
    \framesubtitle{Quantized electromagnetic field}
    
    \begin{columns}
        \begin{column}{0.5\textwidth}
            \center{\textbf{Classical}}
            \begin{equation*}\begin{split}
                \pmb{e}(\pmb{r},t)&=-\sum_n p_n (t)\pmb{u}_n (\pmb{r})\\
                \pmb{h}(\pmb{r},t)&=\sum_n q_n (t)\nabla\times\pmb{u}_n (\pmb{r})\\
                with\ &\pmb{u}_n (\pmb{r})=\pmb{u}_{n0}\ e^{i\pmb{k}_n \cdot \pmb{r}}
            \end{split}\end{equation*}
            \vspace{2.5mm}
            \begin{equation*}\begin{split}
                &H_n=\hbar\omega_n\absolutevalue{a_n(t)}^2\\
                &a_n(t)=\frac{\omega_nq_n(t)+ip_n(t)}{\sqrt{2\hbar\omega_n}}
            \end{split}\end{equation*}
        \end{column}
        \begin{column}{0.5\textwidth}
            \center{\textbf{Quantized}}
            \begin{equation*}\begin{split}
                p_n (t) \implies& P_n(t):\Hilbert\rightarrow\Hilbert\\
                q_n (t) \implies& Q_n(t):\Hilbert\rightarrow\Hilbert\\
                \commutator{\pmb{Q}_n}{\pmb{P}_m}&=i\hbar\delta_{n,m}\pmb{I}\\ 
                \commutator{\pmb{Q}_n}{\pmb{Q}_m}&=0\\
                \commutator{\pmb{P}_n}{\pmb{P}_m}&=0
            \end{split}\end{equation*}
            \begin{equation*}\begin{split}
                &H_n=\hbar\omega_n\pmb{A}_n^\dagger\pmb{A}_n\\
                &\pmb{A}_n(t)=\frac{\omega_n\pmb{Q}_n(t)-i\pmb{P}_n(t)}{\sqrt{2\hbar\omega_n}}
            \end{split}\end{equation*}
        \end{column}
    \end{columns}
    \mbox{}\\
    \mbox{}\\
    \mbox{}\\
    \mbox{}\\
\end{frame}